lambda2Gmu/Infrastructure.v
@@ -1,0 +1,91 @@
+Require Import Definitions.
+Require Import TLC.LibLN.
+
+Hint Constructors type term wft typing red.
+
+Hint Resolve typing_var typing_app typing_tapp.
+
+(** Gathering free names already used in the proofs *)
+Ltac gather_vars :=
+  let A := gather_vars_with (fun x : vars => x) in
+  let B := gather_vars_with (fun x : var => \{x}) in
+  let C := gather_vars_with (fun x : trm => fv_trm x) in
+  let E := gather_vars_with (fun x : typ => fv_typ x) in
+  let F := gather_vars_with (fun x : ctx => dom x) in
+  constr:(A \u B \u C \u E \u F).
+
+(** "pick_fresh x" tactic create a fresh variable with name x *)
+
+Ltac pick_fresh x :=
+  let L := gather_vars in (pick_fresh_gen L x).
+
+(** "apply_fresh T as x" is used to apply inductive rule which
+   use an universal quantification over a cofinite set *)
+
+Tactic Notation "apply_fresh" constr(T) "as" ident(x) :=
+  apply_fresh_base T gather_vars x.
+
+Tactic Notation "apply_fresh" "*" constr(T) "as" ident(x) :=
+  apply_fresh T as x; auto_star.
+
+Ltac get_env :=
+  match goal with
+  | |- wft ?E _ => E
+  | |- typing ?E _ _ => E
+  end.
+
+(* (** These tactics help applying a lemma which conclusion mentions *)
+(*   an environment (E & F) in the particular case when F is empty *) *)
+(* Tactic Notation "apply_empty_bis" tactic(get_env) constr(lemma) := *)
+(*   let E := get_env in rewrite <- (concat_empty E); *)
+(*   eapply lemma; try rewrite concat_empty. *)
+
+(* Tactic Notation "apply_empty" constr(F) := *)
+(*   apply_empty_bis (get_env) F. *)
+
+(* Tactic Notation "apply_empty" "*" constr(F) := *)
+(*   apply_empty F; auto*. *)
+
+Ltac unsimpl_map_bind :=
+  match goal with |- context [ ?B (subst_tt ?Z ?P ?U) ] =>
+    unsimpl ((subst_tb Z P) (B U)) end.
+
+Tactic Notation "unsimpl_map_bind" "*" :=
+  unsimpl_map_bind; auto_star.
+
+(** Substitution for a fresh name is identity. *)
+Lemma subst_tt_fresh : forall Z U T,
+  Z \notin fv_typ T -> subst_tt Z U T = T.
+Proof.
+  induction T; simpl; intros; f_equal*.
+  case_var*.
+Qed.
+
+
+(* TODO *)
+
+(** * Properties of well-formedness of a type in an environment *)
+
+(** If a type is well-formed in an environment then it is locally closed. *)
+
+Lemma type_from_wft : forall Σ E T,
+  wft Σ E T -> type T.
+Proof.
+  induction 1; eauto.
+Qed.
+
+(* Lemma wft_weaken : forall Σ G T E F, *)
+(*   wft Σ (E & G) T -> *)
+(*   ok (E & F & G) -> *)
+(*   wft Σ (E & F & G) T. *)
+(*   intros. *)
+(*   induction H; intros; subst; eauto. *)
+
+(*   - (* fvar *) *)
+(*     econstructor. *)
+(*     admit. *)
+
+(*   - (* all *) *)
+(*     econstructor. *)
+(*     admit. *)
+(* Admitted. *)
