lambda2Gmu/Tests.v
@@ -1,5 +1,6 @@
 Require Import Definitions.
 Require Import TLC.LibLN.
+Require Import Infrastructure.
 
 Notation "@ n" := (typ_bvar n) (at level 42).
 Notation "# n" := (trm_bvar n) (at level 42).
@@ -7,15 +8,15 @@ Notation "# n" := (trm_bvar n) (at level 42).
 Definition id := trm_tabs (trm_abs (@0) (#0)).
 Definition id_typ := typ_all (typ_arrow (@0) (@0)).
 
-Hint Constructors type term wft typing red.
 
 Inductive evals : trm -> trm -> Prop :=
 | eval_step : forall a b c, a --> b -> evals b c -> evals a c
 | eval_finish : forall a, evals a a.
 
 
-Ltac simpl_subst := cbv; try case_if; auto.
-Ltac solve_simple_type := repeat (econstructor; eauto; cbv; try case_if; eauto).
+Ltac simpl_op := cbn; try case_if; auto.
+Ltac solve_simple_type := repeat ((* let L := gather_vars in try apply typing_abs with L; *) econstructor; eauto; cbn; try case_if; eauto).
+Ltac crush_simple_type := repeat (cbv; (try case_if); econstructor; eauto).
 Ltac fs := exact \{}. (* There must be a better way *)
 
 Lemma well_formed_id :
@@ -30,22 +31,32 @@ Lemma well_typed_id : {empty, empty} ⊢ id ∈ id_typ.
   solve_simple_type.
 Qed.
 
+(* Ltac tst := *)
+(*   match goal with *)
+(*   | H: ?x \notin ?L |- _ => instantiate (1 := \{}) *)
+(*   end. *)
+(* Ltac tst := *)
+(*   match goal with *)
+(*   | _:_ |- {?Σ, ?E} ⊢ (trm_abs ?T1 ?e1) open_te_var ?x ∈ (?T open_tt_var ?x) => *)
+(*     instantiate (1 := T1 ==> _) *)
+(*   end. *)
+
 (* TODO we need an ADT for some Nat numbers type *)
 Definition id_id_app := (trm_app (trm_tapp id id_typ) id).
 Lemma id_of_id_types : {empty, empty} ⊢ id_id_app ∈ id_typ.
-  cbv.
-  repeat (econstructor; eauto).
+  solve_simple_type.
   - intros.
     (* instantiate (1 := _ ==> _). *)
     instantiate (1 := (@0) ==> @0).
-    solve_simple_type.
+    simpl_op.
+    crush_simple_type.
   - intros.
     instantiate (1 := (@0) ==> @0).
-    solve_simple_type.
-  - simpl_subst.
+    crush_simple_type.
+  - simpl_op.
 Qed.
 
-Ltac crush_eval := repeat (try (apply eval_finish; eauto); econstructor; simpl_subst).
+Ltac crush_eval := repeat (try (apply eval_finish; eauto); econstructor; simpl_op).
 
 Lemma id_of_id_evals : evals id_id_app id.
   crush_eval.
